2. $x^2 y'' - 20y = 0$
    
    This differential equation is of the form:
    
    $x^2 y'' + axy' + by = 0$
    
    The characteristic equation for this differential equation is:
    
    $m^2 + (a-1)m + b = 0$
    
    For this problem:
    
    $m^2 - m - 20 = 0$
    
    Solving the quadratic equation:
    
    $(m+4)(m-5) = 0$
    
    $m = -4, 5$
    
    Therefore, the solution is:
    
    $y = c_1 x^{-4} + c_2 x^5$

3. $5x^2 y'' + 23xy' + 16.2y = 0$
    
    This differential equation is of the form:
    
    $x^2 y'' + axy' + by = 0$
    
    The characteristic equation for this differential equation is:
    
    $m^2 + (a-1)m + b = 0$
    
    For this problem:
    
    $m^2 + 3.6m + 3.24 = 0$
    
    Solving the quadratic equation:
    
    $m = -1.8$ (repeated root)
    
    Therefore, the solution is:
    
    $y = (c_1 + c_2 \ln x) x^{-1.8}$

4. $xy'' + 2y' = 0$
    
    Multiplying both sides by $x$ to transform it:
    
    $x^2 y'' + 2xy' = 0$
    
    This differential equation is of the form:
    
    $x^2 y'' + axy' + by = 0$
    
    The characteristic equation for this differential equation is:
    
    $m^2 + (a-1)m + b = 0$
    
    For this problem:
    
    $m^2 + m = 0$
    
    Solving the quadratic equation:
    
    $m = 0, -1$
    
    Therefore, the solution is:
    
    $y = c_1 + \frac{c_2}{x}$

5. $4x^2 y'' + 5y = 0$
    
    This differential equation is of the form:
    
    $x^2 y'' + axy' + by = 0$
    
    The characteristic equation for this differential equation is:
    
    $m^2 + (a-1)m + b = 0$
    
    For this problem:
    
    $m^2 - m + \frac{5}{4} = 0$
    
    Solving the quadratic equation:
    
    $m = \frac{1}{2} \pm i$
    
    Therefore, the solution is:
    
    $y = x^{1/2} \{ c_1 \sin (\ln x) + c_2 \cos (\ln x) \}$

6. $x^2 y'' + 0.7xy' - 0.1y = 0$
    
    This differential equation is of the form:
    
    $x^2 y'' + axy' + by = 0$
    
    The characteristic equation for this differential equation is:
    
    $m^2 + (a-1)m + b = 0$
    
    For this problem:
    
    $m^2 - 0.3m - 0.1 = 0$
    
    Solving the quadratic equation:
    
    $m = 0.5, -0.2$
    
    Therefore, the solution is:
    
    $y = c_1 x^{0.5} + c_2 x^{-0.2}$

12. $x^2 y'' - 4xy' + 6y = 0$, $y(1) = 0.4$, $y'(1) = 0$
    
    The characteristic equation for this differential equation is:
    
    $m^2 + (-4-1)m + 6 = 0$
    
    Solving the quadratic equation:
    
    $m^2 - 5m + 6 = 0$
    
    $m = 2, 3$
    
    Therefore, the solution is:
    
    $y = c_1 x^2 + c_2 x^3$
    
    Using the initial conditions:
    
    $y(1) = 0.4 \Rightarrow c_1 + c_2 = 0.4$
    
    $y'(1) = 0 \Rightarrow 2c_1 + 3c_2 = 0$
    
    Solving the system:
    
    $c_1 = 1.2, c_2 = -0.8$
    
    Therefore, the solution is:
    
    $y = 1.2 x^2 - 0.8 x^3$

13. $x^2 y'' + 3xy' + 0.75y = 0$, $y(1) = 1$, $y'(1) = -1.5$
    
    The characteristic equation for this differential equation is:
    
    $m^2 + 2m + 0.75 = 0$
    
    Solving the quadratic equation:
    
    $m = -\frac{3}{2}, -\frac{1}{2}$
    
    Therefore, the solution is:
    
    $y = c_1 x^{-\frac{3}{2}} + c_2 x^{-\frac{1}{2}}$
    
    Using the initial conditions:
    
    $y(1) = 1 \Rightarrow c_1 + c_2 = 1$
    
    $y'(1) = -1.5 \Rightarrow -\frac{3}{2} c_1 - \frac{1}{2} c_2 = -1.5$
    
    Solving the system:
    
    $c_1 = 1, c_2 = 0$
    
    Therefore, the solution is:
    
    $y = x^{-\frac{3}{2}}$

14. $x^2 y'' + xy' + 9y = 0$, $y(1) = 0$, $y'(1) = 2.5$
    
    The characteristic equation for this differential equation is:
    
    $m^2 + 9 = 0$
    
    Solving the quadratic equation:
    
    $m = \pm 3i$
    
    Therefore, the solution is:
    
    $y = c_1 \sin (3 \ln x) + c_2 \cos (3 \ln x)$
    
    Using the initial conditions:
    
    $y(1) = 0 \Rightarrow c_2 = 0$
    
    $y'(1) = 2.5 \Rightarrow 3c_1 = 2.5 \Rightarrow c_1 = \frac{2.5}{3}$
    
    Therefore, the solution is:
    
    $y = \frac{2.5}{3} \sin (3 \ln x)$

15. $x^2 y'' + 3xy' + y = 0$, $y(1) = 3.6$, $y'(1) = 0.4$
    
    The characteristic equation for this differential equation is:
    
    $m^2 + 2m + 1 = 0$
    
    Solving the quadratic equation:
    
    $m = -1$ (repeated root)
    
    Therefore, the solution is:
    
    $y = (c_1 + c_2 \ln x) x^{-1}$
    
    Using the initial conditions:
    
    $y(1) = 3.6 \Rightarrow c_1 + c_2 = 3.6$
    
    $y'(1) = 0.4 \Rightarrow -c_1 - c_2 = -0.4$
    
    Solving the system:
    
    $c_1 = -0.4, c_2 = 4$
    
    Therefore, the solution is:
    
    $y = (-0.4 + 4 \ln x) x^{-1}$


