1. $4y'' - 25y = 0$
    
    This is of the form $ay'' + by' + cy = 0$, which has solutions of the form $e^{\lambda x}$.
    
    Solving the characteristic equation:
    
    $4\lambda^2 - 25 = 0$
    
    $\lambda = \pm \frac{5}{2}$
    
    Therefore, the solution is $y = c_1 e^{2.5 x} + c_2 e^{-2.5 x}$.

2. $y'' + 36 y = 0$
    
    This is of the form $ay'' + by' + cy = 0$, which has solutions of the form $e^{\lambda x}$.
    
    Solving the characteristic equation:
    
    $\lambda^2 + 36 = 0$
    
    $\lambda = \pm 6i$
    
    The general solution for complex roots is:
    
    $y = c_1 \cos 6x + c_2 \sin 6x$

3. $y'' + 6y' + 8.96 y = 0$
    
    This is of the form $ay'' + by' + cy = 0$, which has solutions of the form $e^{\lambda x}$.
    
    Solving the characteristic equation:
    
    $\lambda^2 + 6\lambda + 8.96 = 0$
    
    $\lambda = -3.2, -2.8$
    
    Therefore, the solution is $y = c_1 e^{-3.2 x} + c_2 e^{-2.8 x}$.

4. $y'' + 4y' + (\pi^2 + 4)y = 0$
    
    This is of the form $ay'' + by' + cy = 0$, which has solutions of the form $e^{\lambda x}$.
    
    Solving the characteristic equation:
    
    $\lambda^2 + 4 \lambda + (\pi^2 + 4) = 0$
    
    $\lambda = -2 \pm \pi i$
    
    Therefore, the solution is:
    
    $y = e^{-2x} \{ c_1 \cos \pi x + c_2 \sin \pi x \}$

5. $y'' + 2\pi y' + \pi y = 0$
    
    This is of the form $ay'' + by' + cy = 0$, which has solutions of the form $e^{\lambda x}$.
    
    Solving the characteristic equation:
    
    $\lambda^2 + 2\pi \lambda + \pi^2 = 0$
    
    $\lambda = -\pi$ (repeated root)
    
    Therefore, the solution is:
    
    $y = (c_1 + c_2 x) e^{-\pi x}$

6. $10 y'' - 32 y' + 25.6 y = 0$
    
    This is of the form $ay'' + by' + cy = 0$, which has solutions of the form $e^{\lambda x}$.
    
    Solving the characteristic equation:
    
    $10 \lambda^2 - 32 \lambda + 25.6 = 0$
    
    $\lambda = 1.6$ (repeated root)
    
    Therefore, the solution is:
    
    $y = (c_1 + c_2 x) e^{1.6x}$

7. $y'' + 4.5 y' = 0$
    
    This is of the form $ay'' + by' + cy = 0$, which has solutions of the form $e^{\lambda x}$.
    
    Solving the characteristic equation:
    
    $\lambda^2 + 4.5 \lambda = 0$
    
    $\lambda = 0, -4.5$
    
    Therefore, the solution is:
    
    $y = c_1 + c_2 e^{-4.5x}$

8. $y'' + y' + 3.25 y = 0$
    
    This is of the form $ay'' + by' + cy = 0$, which has solutions of the form $e^{\lambda x}$.
    
    Solving the characteristic equation:
    
    $\lambda^2 + \lambda + 3.25 = 0$
    
    $\lambda = -\frac{1}{2} \pm \sqrt{12} i$
    
    Therefore, the solution is:
    
    $y = e^{-\frac{1}{2}x} \{ c_1 \cos (\sqrt{12}x) + c_2 \sin (\sqrt{12} x) \}$

9. $y'' + 1.8 y' - 2.08 y = 0$
    
    This is of the form $ay'' + by' + cy = 0$, which has solutions of the form $e^{\lambda x}$.
    
    Solving the characteristic equation:
    
    $\lambda^2 + 1.8 \lambda - 2.08 = 0$
    
    $\lambda = 2.6, -0.8$
    
    Therefore, the solution is:
    
    $y = c_1 e^{2.6x} + c_2 e^{-0.8x}$

10. $100y'' + 240 y' + (196\pi^2 + 144) = 0$
    
    This is of the form $ay'' + by' + cy = 0$, which has solutions of the form $e^{\lambda x}$.
    
    Solving the characteristic equation:
    
    $100 \lambda^2 + 240 \lambda + (196 \pi^2 + 144) = 0$
    
    $\lambda = -1.2 \pm 1.4 \pi i$
    
    Therefore, the solution is:
    
    $y = e^{-1.2x} \{ c_1 \cos (1.4 \pi x) + c_2 \sin (1.4 \pi x) \}$

11. $4y'' - 4y' - 3y = 0$
    
    This is of the form $ay'' + by' + cy = 0$, which has solutions of the form $e^{\lambda x}$.
    
    Solving the characteristic equation:
    
    $4 \lambda^2 - 4\lambda - 3 = 0$
    
    $\lambda = \frac{3}{2}, -\frac{1}{2}$
    
    Therefore, the solution is:
    
    $y = c_1 e^{\frac{3}{2}x} + c_2 e^{-\frac{1}{2}x}$

12. $y'' + 9y' + 20 y = 0$
    
    This is of the form $ay'' + by' + cy = 0$, which has solutions of the form $e^{\lambda x}$.
    
    Solving the characteristic equation:
    
    $\lambda^2 + 9\lambda + 20 = 0$
    
    $\lambda = -4, -5$
    
    Therefore, the solution is:
    
    $y = c_1 e^{-4x} + c_2 e^{-5x}$

13. $9y'' - 30 y' + 25y = 0$
    
    This is of the form $ay'' + by' + cy = 0$, which has solutions of the form $e^{\lambda x}$.
    
    Solving the characteristic equation:
    
    $9 \lambda^2 - 30 \lambda + 25 = 0$
    
    $\lambda = \frac{5}{3}$ (repeated root)
    
    Therefore, the solution is:
    
    $y = (c_1 + c_2 x) e^{\frac{5}{3}x}$

14. $y'' + 2k^2 y' + k^4 y = 0$
    
    This is of the form $ay'' + by' + cy = 0$, which has solutions of the form $e^{\lambda x}$.
    
    Solving the characteristic equation:
    
    $\lambda^2 + 2k^2 \lambda + k^4 = 0$
    
    $\lambda = -k^2$ (repeated root)
    
    Therefore, the solution is:
    
    $y = (c_1 + c_2 x) e^{-k^2 x}$

15. $y'' + 0.54 y' + (0.0729 + \pi) y = 0$
    
    This is of the form $ay'' + by' + cy = 0$, which has solutions of the form $e^{\lambda x}$.
    
    Solving the characteristic equation:
    
    $\lambda^2 + 0.54 \lambda + (0.0729 + \pi) = 0$
    
    $\lambda = -0.27 \pm \sqrt{\pi} i$
    
    Therefore, the solution is:
    
    $y = e^{-0.27x} (c_1 \cos \sqrt{\pi} x + c_2 \sin \sqrt{\pi} x)$

21. $y'' + 25 y = 0$, $y(0) = 4.6$ , $y'(0) = -1.2$

    This is of the form $ay'' + by' + cy = 0$, which has solutions of the form $e^{\lambda x}$.
    
    Solving the characteristic equation:
    
    $\lambda^2 + 25 = 0$
    
    $\lambda = \pm 5i$
    
    Therefore, the solution is:
    
    $y = c_1 \cos 5x + c_2 \sin 5x$
    
    Using the initial conditions:
    
    $y(0) = 4.6 \Rightarrow c_1 = 4.6$
    
    $y'(0) = -1.2 \Rightarrow 5c_2 = -1.2 \Rightarrow c_2 = -0.24$
    
    Therefore, the solution is:
    
    $y = 4.6 \cos 5x - 0.24 \sin 5x$

23. $y'' + y' - 6y = 0$, $y(0) = 10$, $y'(0) = 0$
    
    This is of the form $ay'' + by' + cy = 0$, which has solutions of the form $e^{\lambda x}$.
    
    Solving the characteristic equation:
    
    $\lambda^2 + \lambda - 6 = 0$
    
    $\lambda = 2, -3$
    
    Therefore, the solution is:
    
    $y = c_1 e^{2x} + c_2 e^{-3x}$
    
    Using the initial conditions:
    
    $y(0) = 10 \Rightarrow c_1 + c_2 = 10$
    
    $y'(0) = 0 \Rightarrow 2c_1 - 3c_2 = 0 \Rightarrow 2c_1 = 3c_2 \Rightarrow c_1 = \frac{3}{2}c_2$
    
    Substituting back:
    
    $\frac{5}{2}c_2 = 10 \Rightarrow c_2 = 4 \Rightarrow c_1 = 6$
    
    Therefore, the solution is:
    
    $y = 6e^{2x} + 4e^{-3x}$

24. $4y'' - 4 y' - 3y = 0$, $y(-2) = e$, $y'(-2) = -\frac{e}{2}$
    
    This is of the form $ay'' + by' + cy = 0$, which has solutions of the form $e^{\lambda x}$.
    
    Solving the characteristic equation:
    
    $4\lambda^2 - 4\lambda - 3 = 0$
    
    $\lambda = \frac{3}{2}, -\frac{1}{2}$
    
    Therefore, the solution is:
    
    $y = c_1 e^{\frac{3}{2} x} + c_2 e^{-\frac{1}{2} x}$
    
    Using the initial conditions:
    
    $y(-2) = e \Rightarrow c_1 e^{-3} + c_2 e = e$
    
    $y'(-2) = -\frac{e}{2} \Rightarrow \frac{3}{2} c_1 e^{-3} - \frac{1}{2} c_2 e = -\frac{e}{2}$
    
    Solving the system:
    
    $c_1 = 0$
    
    $c_2 = 1$
    
    Therefore, the solution is:
    
    $y = e^{-\frac{1}{2} x}$

25. $y'' - y = 0$, $y(0) = 2$, $y'(0) = -2$
    
    This is of the form $ay'' + by' + cy = 0$, which has solutions of the form $e^{\lambda x}$.
    
    Solving the characteristic equation:
    
    $\lambda^2 - 1 = 0$
    
    $\lambda = \pm 1$
    
    Therefore, the solution is:
    
    $y = c_1 e^x + c_2 e^{-x}$
    
    Using the initial conditions:
    
    $y(0) = 2 \Rightarrow c_1 + c_2 = 2$
    
    $y'(0) = -2 \Rightarrow c_1 - c_2 = -2$
    
    Solving the system:
    
    $c_1 = 0, c_2 = 2$
    
    Therefore, the solution is:
    
    $y = 2e^{-x}$

26. $y'' - k^2 y = 0$, $y(0) = 1$, $y'(0) = 1$
    
    This is of the form $ay'' + by' + cy = 0$, which has solutions of the form $e^{\lambda x}$.
    
    Solving the characteristic equation:
    
    $\lambda^2 - k^2 = 0$
    
    $\lambda = \pm k$
    
    Therefore, the solution is:
    
    $y = c_1 e^{kx} + c_2 e^{-kx}$
    
    Using the initial conditions:
    
    $y(0) = 1 \Rightarrow c_1 + c_2 = 1$
    
    $y'(0) = 1 \Rightarrow k c_1 - k c_2 = 1$
    
    Solving the system:
    
    $c_1 = \frac{e^k (k + 1)}{2k}$
    
    $c_2 = \frac{e^k (k - 1)}{2k}$
    
    Therefore, the solution is:
    
    $y = \frac{e^k (k + 1)}{2k} e^{kx} + \frac{e^k (k - 1)}{2k} e^{-kx}$

28. $8y'' - 2y' - y = 0$, $y(0) = -0.2$, $y'(0) = -0.325$

    This is of the form $ay'' + by' + cy = 0$, which has solutions of the form $e^{\lambda x}$.
    
    Solving the characteristic equation:
    
    $8 \lambda^2 - 2\lambda - 1 = 0$
    
    $\lambda = -\frac{1}{4}, \frac{1}{2}$
    
    Therefore, the solution is:
    
    $y = c_1 e^{-\frac{1}{4}x} + c_2 e^{\frac{1}{2}x}$
    
    Using the initial conditions:
    
    $y(0) = -0.2 \Rightarrow c_1 + c_2 = -0.2$
    
    $y'(0) = -0.325 \Rightarrow -\frac{1}{4}c_1 + \frac{1}{2}c_2 = -0.325$
    
    Solving the system:
    
    $c_1 = 0.3$
    
    $c_2 = -0.5$
    
    Therefore, the solution is:
    
    $y = 0.3 e^{-\frac{1}{4}x} - 0.5 e^{\frac{1}{2}x}$

30. $9y'' - 30y' + 25y = 0$, $y(0) = 3.3$, $y'(0) = 10$
    
    This is of the form $ay'' + by' + cy = 0$, which has solutions of the form $e^{\lambda x}$.
    
    Solving the characteristic equation:
    
    $9 \lambda^2 - 30 \lambda + 25 = 0$
    
    $\lambda = \frac{5}{3}$ (repeated root)
    
    Therefore, the solution is:
    
    $y = (c_1 + c_2 x) e^{\frac{5}{3}x}$
    
    Using the initial conditions:
    
    $y(0) = 3.3 \Rightarrow c_1 = 3.3$
    
    $y'(0) = 10 \Rightarrow \frac{5}{3} c_1 + c_2 = 10 \Rightarrow c_2 = 4.5$
    
    Therefore, the solution is:
    
    $y = (3.3 + 4.5 x) e^{\frac{5}{3}x}$

